



PRÁCTICA CALIFICADA 1

Apellidos y Nombres :
Docente : Dra. Zayda Villanueva Vega
Fecha : viernes 12, setiembre, 2025.

1. (7 puntos) Halle si existe $\lim_{x \rightarrow 27} \frac{\sqrt{6 + \sqrt[3]{x}} - 3}{x^2 - 27x}$

SOLUCION

$$\lim_{x \rightarrow 27} \frac{\sqrt{6 + \sqrt[3]{x}} - 3}{x^2 - 27x} = \lim_{x \rightarrow 27} \frac{(\sqrt{6 + \sqrt[3]{x}} - 3)(\sqrt{6 + \sqrt[3]{x}} + 3)}{x(x - 27)(\sqrt{6 + \sqrt[3]{x}} + 3)}$$

$$\lim_{x \rightarrow 27} \frac{\sqrt{6 + \sqrt[3]{x}} - 3}{x^2 - 27x} = \lim_{x \rightarrow 27} \frac{(\sqrt[3]{x} - 3)}{x(x - 27)} = \lim_{x \rightarrow 27} \frac{(\sqrt[3]{x} - 3)(\sqrt[3]{x^2} + 3\sqrt[3]{x} + 9)}{x(x - 27)(\sqrt{6 + \sqrt[3]{x}} + 3)(\sqrt[3]{x^2} + 3\sqrt[3]{x} + 9)}$$

$$\lim_{x \rightarrow 27} \frac{\sqrt{6 + \sqrt[3]{x}} - 3}{x^2 - 27x} = \lim_{x \rightarrow 27} \frac{(\sqrt[3]{x} - 3)}{x(x - 27)} = \lim_{x \rightarrow 27} \frac{(\sqrt[3]{x} - 3)(\sqrt[3]{x^2} + 3\sqrt[3]{x} + 9)}{x(x - 27)(\sqrt{6 + \sqrt[3]{x}} + 3)(\sqrt[3]{x^2} + 3\sqrt[3]{x} + 9)}$$

$$\lim_{x \rightarrow 27} \frac{\sqrt{6 + \sqrt[3]{x}} - 3}{x^2 - 27x} = \lim_{x \rightarrow 27} \frac{(x - 27)}{x(x - 27)(\sqrt{6 + \sqrt[3]{x}} + 3)(\sqrt[3]{x^2} + 3\sqrt[3]{x} + 9)}$$

$$\lim_{x \rightarrow 27} \frac{\sqrt{6 + \sqrt[3]{x}} - 3}{x^2 - 27x} = \lim_{x \rightarrow 27} \frac{1}{x(\sqrt{6 + \sqrt[3]{x}} + 3)(\sqrt[3]{x^2} + 3\sqrt[3]{x} + 9)}$$

$$\lim_{x \rightarrow 27} \frac{\sqrt{6 + \sqrt[3]{x}} - 3}{x^2 - 27x} = \lim_{x \rightarrow 27} \frac{1}{x(\sqrt{6 + \sqrt[3]{x}} + 3)(\sqrt[3]{x^2} + 3\sqrt[3]{x} + 9)}$$

$$\lim_{x \rightarrow 27} \frac{\sqrt{6 + \sqrt[3]{x}} - 3}{x^2 - 27x} = \frac{1}{27(6)(27)}$$

$$\lim_{x \rightarrow 27} \frac{\sqrt{6 + \sqrt[3]{x}} - 3}{x^2 - 27x} = \frac{1}{4374}$$

2. **(6 puntos)** Halle si existe $\lim_{x \rightarrow 1} \frac{3 - |x - 1|}{2|x - 1| + 3}$

SOLUCION

$$\frac{3 - |x - 1|}{2|x - 1| + 3} = \begin{cases} \frac{3 - (x - 1)}{2(x - 1) + 3}; & x - 1 \geq 0 \\ \frac{3 - (-x + 1)}{2(-x + 1) + 3}; & x - 1 < 0 \end{cases}$$

$$\frac{3 - |x - 1|}{2|x - 1| + 3} = \begin{cases} \frac{4 - x}{2x + 1}; & x \geq 1 \\ \frac{2 + x}{-2x + 5}; & x < 1 \end{cases}$$

$$\lim_{x \rightarrow 1^+} \frac{3 - |x - 1|}{2|x - 1| + 3} = \lim_{\substack{x \rightarrow 1 \\ x > 1}} \frac{4 - x}{2x + 1} = \frac{3}{3} = 1$$

$$\lim_{x \rightarrow 1^-} \frac{3 - |x - 1|}{2|x - 1| + 3} = \lim_{\substack{x \rightarrow 1 \\ x < 1}} \frac{2 + x}{-2x + 5} = \frac{3}{3} = 1$$

$$\therefore \exists \lim_{x \rightarrow 1} \frac{3 - |x - 1|}{2|x - 1| + 3} = 1$$

3. (7 puntos) Halle si existe $\lim_{x \rightarrow 0} \frac{2 - \sqrt{\cos(\operatorname{sen}(2x))} - \sqrt{1 - \operatorname{sen}^2 x}}{x^2 \cos x}$

SOLUCION

$$\lim_{x \rightarrow 0} \frac{2 - \sqrt{\cos(\operatorname{sen}(2x))} - \sqrt{1 - \operatorname{sen}^2 x}}{x^2 \cos x} = \lim_{x \rightarrow 0} \frac{\left(1 - \sqrt{\cos(\operatorname{sen}(2x))}\right) + (1 - \cos x)}{x^2 \cos x}$$

$$= \lim_{x \rightarrow 0} \frac{\left(1 - \sqrt{\cos(\operatorname{sen}(2x))}\right)}{x^2 \cos x} + \frac{1 - \cos x}{x^2 \cos x}$$

$$= \lim_{x \rightarrow 0} \frac{\left(1 - \sqrt{\cos(\operatorname{sen}(2x))}\right)\left(1 + \sqrt{\cos(\operatorname{sen}(2x))}\right)}{x^2 \cos x \left(1 + \sqrt{\cos(\operatorname{sen}(2x))}\right)} + \frac{1 - \cos x}{x^2} \cdot \frac{1}{\cos x}$$

$$= \lim_{x \rightarrow 0} \frac{\frac{1 - (\cos(\operatorname{sen}(2x)))}{\operatorname{sen}^2(2x)}}{\frac{x^2}{\operatorname{sen}^2(2x)} \cdot \left(1 + \sqrt{\cos(\operatorname{sen}(2x))}\right)} + \frac{1 - \cos x}{x^2} \cdot \frac{1}{\cos x}$$

$$= \lim_{x \rightarrow 0} \frac{4 \frac{\operatorname{sen}^2(2x)}{4x^2} \cdot \frac{1 - (\cos(\operatorname{sen}(2x)))}{\operatorname{sen}^2(2x)}}{\left(1 + \sqrt{\cos(\operatorname{sen}(2x))}\right)} + \frac{1 - \cos x}{x^2} \cdot \frac{1}{\cos x}$$

$$= \lim_{x \rightarrow 0} \frac{4 \cdot \frac{\operatorname{sen}(2x)}{2x} \cdot \frac{\operatorname{sen}(2x)}{2x} \cdot \frac{1 - (\cos(\operatorname{sen}(2x)))}{\operatorname{sen}^2(2x)}}{\left(1 + \sqrt{\cos(\operatorname{sen}(2x))}\right)} + \frac{1 - \cos x}{x^2} \cdot \frac{1}{\cos x}$$

$$= \frac{4(1)(1)\left(\frac{1}{2}\right)}{(2)} + \frac{1}{2} \cdot 1$$

$$\lim_{x \rightarrow 0} \frac{2 - \sqrt{\cos(\operatorname{sen}(2x))} - \sqrt{1 - \operatorname{sen}^2 x}}{x^2 \cos x} = \frac{3}{2}$$